pulse/share/steel/examples/pulse/lib/PulseHashTable.fsti
@@ -46,10 +46,15 @@ type locked_ht_t (s:pht_sig_us) = ht:ht_t s & LK.lock (exists_ (fun pht -> model
 
 let pht_sz #s (pht:pht_t s) : pos = pht.sz
 
+let destroy_val_fn_t (t:Type0) : Type = v:t -> stt unit emp (fun _ -> emp) 
 
 
 val alloc_locked (#s:pht_sig_us) (l:pos_us)
   : stt (locked_ht_t s) emp (fun _ -> emp)
+
+val dealloc (#s:pht_sig_us) (ht:ht_t s) (l:pos_us) (destroy_val:destroy_val_fn_t s.valt)
+  : stt unit (requires exists_ (fun pht -> models s ht pht))
+             (ensures fun _ -> emp)
 
 val lookup (#s:pht_sig_us)
            (#pht:erased (pht_t (s_to_ps s)))
